rubin-formal/RubinFormal/CovenantRegistryExhaustive.lean
@@ -26,7 +26,6 @@ def covenantDisposition (tag : Nat) : CovenantDisposition :=
   else if tag = 0x00FF then CovenantDisposition.reserved
   else if tag = 0x0100 then CovenantDisposition.accepted CovenantKind.coreHTLC
   else if tag = 0x0101 then CovenantDisposition.accepted CovenantKind.coreVault
-  else if tag = 0x0102 then CovenantDisposition.invalidCovenantType
   else if tag = 0x0103 then CovenantDisposition.accepted CovenantKind.coreDACommit
   else if tag = 0x0104 then CovenantDisposition.accepted CovenantKind.coreMultisig
   else if tag = 0x0105 then CovenantDisposition.accepted CovenantKind.coreStealth
@@ -42,13 +41,12 @@ def section14DispositionCase (tag : Nat) (disposition : CovenantDisposition) : P
     (tag = 0x00FF ∧ disposition = CovenantDisposition.reserved) ∨
     (tag = 0x0100 ∧ disposition = CovenantDisposition.accepted CovenantKind.coreHTLC) ∨
     (tag = 0x0101 ∧ disposition = CovenantDisposition.accepted CovenantKind.coreVault) ∨
-    (tag = 0x0102 ∧ disposition = CovenantDisposition.invalidCovenantType) ∨
     (tag = 0x0103 ∧ disposition = CovenantDisposition.accepted CovenantKind.coreDACommit) ∨
     (tag = 0x0104 ∧ disposition = CovenantDisposition.accepted CovenantKind.coreMultisig) ∨
     (tag = 0x0105 ∧ disposition = CovenantDisposition.accepted CovenantKind.coreStealth) ∨
     (tag = 0x0106 ∧ disposition = CovenantDisposition.deploymentGated CovenantKind.coreSimplicity) ∨
     (tag ≠ 0x0000 ∧ tag ≠ 0x0001 ∧ tag ≠ 0x0002 ∧ tag ≠ 0x00FF ∧
-      tag ≠ 0x0100 ∧ tag ≠ 0x0101 ∧ tag ≠ 0x0102 ∧ tag ≠ 0x0103 ∧
+      tag ≠ 0x0100 ∧ tag ≠ 0x0101 ∧ tag ≠ 0x0103 ∧
       tag ≠ 0x0104 ∧ tag ≠ 0x0105 ∧ tag ≠ 0x0106 ∧
       disposition = CovenantDisposition.invalidCovenantType))
 
@@ -70,23 +68,20 @@ theorem covenantDispositionComplete (tag : Nat) (hU16 : tag < 0x10000) :
   · simp [covenantDisposition, hP2PK, hInvalidOne, hAnchor, hReserved, hHtlc]
   by_cases hVault : tag = 0x0101
   · simp [covenantDisposition, hP2PK, hInvalidOne, hAnchor, hReserved, hHtlc, hVault]
-  by_cases hInvalidTwo : tag = 0x0102
-  · simp [covenantDisposition, hP2PK, hInvalidOne, hAnchor, hReserved, hHtlc, hVault,
-      hInvalidTwo]
   by_cases hDaCommit : tag = 0x0103
   · simp [covenantDisposition, hP2PK, hInvalidOne, hAnchor, hReserved, hHtlc, hVault,
-      hInvalidTwo, hDaCommit]
+      hDaCommit]
   by_cases hMultisig : tag = 0x0104
   · simp [covenantDisposition, hP2PK, hInvalidOne, hAnchor, hReserved, hHtlc, hVault,
-      hInvalidTwo, hDaCommit, hMultisig]
+      hDaCommit, hMultisig]
   by_cases hStealth : tag = 0x0105
   · simp [covenantDisposition, hP2PK, hInvalidOne, hAnchor, hReserved, hHtlc, hVault,
-      hInvalidTwo, hDaCommit, hMultisig, hStealth]
+      hDaCommit, hMultisig, hStealth]
   by_cases hSimplicity : tag = 0x0106
   · simp [covenantDisposition, hP2PK, hInvalidOne, hAnchor, hReserved, hHtlc, hVault,
-      hInvalidTwo, hDaCommit, hMultisig, hStealth, hSimplicity]
+      hDaCommit, hMultisig, hStealth, hSimplicity]
   · simp [covenantDisposition, hP2PK, hInvalidOne, hAnchor, hReserved, hHtlc, hVault,
-      hInvalidTwo, hDaCommit, hMultisig, hStealth, hSimplicity]
+      hDaCommit, hMultisig, hStealth, hSimplicity]
 
 private def repeatByte (b : UInt8) (n : Nat) : Bytes :=
   Id.run <| do
